Substantial rewrite + progress

src/register_machine.lean
@@ -1,86 +1,26 @@
+import data.fin
+import data.fin2
+import data.fintype.fin
+import data.equiv.encodable.basic
+import data.list
+import data.matrix.notation
+import data.nat.log
+import data.nat.pairing
+import data.pfun
 import data.vector
 import data.vector2
-import data.equiv.encodable.basic
-import data.fin
-import data.nat.pairing
-import data.nat.log
+import init.data.nat.basic
 import logic.function.iterate
 
-/- for printing out register machines reasonably. should be autoderived but ?? whatever -/
-instance {α : Type*} [has_repr α] {len : ℕ} : has_repr (vector α len)
-  := {repr := λ v, repr v.to_list}
+instance encodable.list {α} [encodable α] : encodable (list α)
+  := ⟨list.rec 0 (λ h _, nat.mkpair (encodable.encode h)),
+      sorry,
+      sorry⟩
 
-@[simp]
-lemma vector.update_nth_eq_if {α : Type*} {len : ℕ} {v : vector α len}
-    {i : fin len} {elem : α} (h : v.nth i = elem)
-  : v.update_nth i elem = v
-  := begin
-    refine vector.ext _,
-    assume m,
-    rw vector.nth_update_nth_eq_if,
-    rw ← h,
-    split_ifs,
-    simp [h_1]
-  end
+instance encodable.fin_tuple {n : ℕ} {α : Type*} [encodable α] : encodable (fin n → α)
+  := encodable.of_equiv (list α) sorry
 
-@[simp]
-lemma vector.update_nth_update_nth_same {α : Type*} {len : ℕ} {v : vector α len}
-    {i : fin len} {e1 e2 : α}
-  : (v.update_nth i e1).update_nth i e2 = v.update_nth i e2
-  := begin
-    refine vector.ext _,
-    assume m,
-    by_cases i=m,
-    rw h,
-    iterate { rw vector.nth_update_nth_same },
-    iterate { rw vector.nth_update_nth_of_ne },
-    iterate { exact h }
-  end
-
-lemma vector.update_nth_comm {α : Type*} {len : ℕ} {v : vector α len}
-    {i j : fin len} {e1 e2 : α} (p : i ≠ j)
-  : (v.update_nth i e1).update_nth j e2 = (v.update_nth j e2).update_nth i e1
-  := begin
-    refine vector.ext _,
-    assume m,
-    by_cases i=m,
-    rw h,
-    rw vector.nth_update_nth_same,
-    rw vector.nth_update_nth_of_ne,
-    rw vector.nth_update_nth_same,
-    rw ← h,
-    exact ne.symm p,
-    by_cases j=m,
-    rw ← h,
-    rw vector.nth_update_nth_same,
-    rw vector.nth_update_nth_of_ne,
-    rw vector.nth_update_nth_same,
-    exact p,
-    iterate {rw vector.nth_update_nth_of_ne},
-    iterate {simp [*]},
-  end
-
-@[simp]
-lemma vector.nth_of_append_fst {α : Type*} {l1 l2 : ℕ} (v1 : vector α l1) (v2 : vector α l2)
-    (i : fin l1) : (v1.append v2).nth (fin.cast_add l2 i) = v1.nth i
-  := begin
-    cases v1,
-    cases v2,
-    exact list.nth_le_append _ _,
-  end
-
-@[simp]
-lemma vector.nth_of_append_snd {α : Type*} {l1 l2 : ℕ} (v1 : vector α l1) (v2 : vector α l2)
-    (i : fin l2) : (v1.append v2).nth (fin.nat_add l1 i) = v2.nth i
-  := begin
-    cases v1,
-    cases v2,
-    simp! [list.nth_le_drop],
-    congr,
-    simp [← v1_property],
-  end
-
-namespace regmachine
+namespace rm
 
 /-  inc r l    ->  increment r and jump to l
     dec r l k  ->  if (r) > 0 then decrement r and jump to l, else jump to k
@@ -110,152 +50,360 @@ variables {rc ic : ℕ}
         instr.inc r' l' := r = r' ∧ loc_eq l l' | _ := ⊥ end 
     | (instr.dec r l k) := λ i, match i with
         instr.dec r' l' k' := r = r' ∧ loc_eq l l' ∧ loc_eq k k' | _ := ⊥ end
+
+  def reg : instr rc ic → fin rc
+    | (instr.inc r _) := r
+    | (instr.dec r _ _) := r
+
+  def equiv_destr : instr rc ic ≃ (fin rc × option (fin ic) ⊕ fin rc × option (fin ic) × option (fin ic))
+    := ⟨(λ i, match i with instr.inc r l := sum.inl (r,l)
+                        | instr.dec r l k := sum.inr (r,l,k) end),
+        (λ i, match i with sum.inl (r,l) := instr.inc r l
+                        | sum.inr (r,l,k) := instr.dec r l k end),
+        begin intro, cases x, iterate {simp [equiv_destr._match_1, equiv_destr._match_2]}, end,
+        begin intro, iterate {cases x, simp [equiv_destr._match_1, equiv_destr._match_2]},
+              cases x_snd, simp [equiv_destr._match_1, equiv_destr._match_2], end⟩
+
+  instance {rc ic : ℕ} : encodable (instr rc ic)
+    := encodable.of_equiv _ equiv_destr
+
 end instr
 
-/- state consists of an instruction pointer and the registers.
-   if ip is none then machine is halted. -/
-structure state (rc ic : ℕ) := (ip : option (fin ic)) (regs : vector ℕ rc)
-namespace state
-  @[simp] def init {rc ic : ℕ} (input : ℕ) : state rc.succ ic.succ
-    := {ip := some 0, regs := input ::ᵥ vector.repeat 0 rc}
-  @[simp] def is_halted {rc ic : ℕ} (s : state rc ic) := s.ip = none
-end state
+/- register machine program with rc registers, ic instructions -/
+@[reducible] def prog (rc ic : ℕ) := fin ic → (instr rc ic)
 
-/- register machine with rc registers and ic instructions -/
-def rm (rc ic : ℕ)
-  := vector (instr rc ic) ic
+/- config consists of an instruction pointer and registers. -/
+structure config (rc ic : ℕ) := (ip : option (fin ic)) (regs : fin rc → ℕ)
+namespace config
+  -- start at instruction 0 if it exists
+  @[simp] def init_ip (rc ic : ℕ) : option (fin ic)
+    := match ic with 0 := none | icp+1 := some 0 end
 
-namespace rm
-  variables {rc ic : ℕ} (M : rm rc ic)
+  -- init register 0 with input, all others with 0
+  @[simp] def init_regs (rcp ic : ℕ) (input : ℕ) : fin rcp.succ → ℕ
+    := fin.cons input (function.const (fin rcp) 0)
+  
+  @[simp] def init {rcp ic : ℕ} (input : ℕ) : config rcp.succ ic
+    :=  {ip := init_ip rcp.succ ic,
+        regs := init_regs rcp ic input }
+  
+  @[simp] def halted {rc ic : ℕ} (regs : fin rc → ℕ) : config rc ic
+    -- output will be at register 0
+    := {ip := none, regs := regs}
 
+  @[reducible] def is_halted {rc ic : ℕ} (c : config rc ic) : Prop
+    := c.ip = none
+
+  /- @[reducible] def is_halted {rc ic : ℕ} (c : config rc ic) := c.ip = none
+  @[reducible] def output {rcp ic : ℕ} (c : config rcp.succ ic) : ℕ ⊕ config rcp.succ ic
+    := if c.is_halted then sum.inl (c.regs 0) else sum.inr c
+
+  theorem ic_zero_is_halted {rc : ℕ} (c : config rc 0) : c.is_halted
+    := begin cases h : c.ip, exact h, exact fin.elim0 val end -/
+end config
+
+namespace prog
+  variables {rc ic : ℕ} (P : prog rc ic)
+  
   /- most important definition here! gives semantics to those incs and decs :) -/
-  def step (c : state rc ic) : state rc ic :=
+  def step (c : config rc ic) :=
     match c.ip with
     | none := c
     | some ip :=
-      match M.nth ip with
-      | instr.inc r l := {ip := l, regs := c.regs.update_nth r (c.regs.nth r + 1)}
+      match P ip with
+      | instr.inc r l := {ip := l, regs := function.update c.regs r (c.regs r + 1)}
       | instr.dec r l k :=
-          match c.regs.nth r with
-          | p + 1 := {ip := l, regs := c.regs.update_nth r p}
+          match c.regs r with
+          | p + 1 := {ip := l, regs := function.update c.regs r p}
           | 0 := {ip := k, regs := c.regs}
           end
       end
     end
-  notation c `[` M `]==>` d := M.step c = d
+
+  notation c `[` P `]==>` d := step P c = d
 
   @[simp]
-  def step_t (t : ℕ) := M.step^[t]
-  notation c `[` M `]==>^[` t `]` d := (M.step_t t) c = d
+  def step_t (t : ℕ)
+    := (step P)^[t]
 
-  def steps_to (c d : state rc ic)
-    := ∃ (t : ℕ), c [M]==>^[t] d
-  notation c `[` M `]==>*` d := M.steps_to c d
+  notation c `[` P `]==>^[` t `]` d := (step_t P t) c = d
+
+  def steps_to (c d : config rc ic)
+    := ∃ (t : ℕ), c [P]==>^[t] d
+
+  notation c `[` P `]==>*` d := steps_to P c d
 
   @[simp]
-  lemma step_is_step_t_1 {c d : state rc ic}
-    : (c [M]==>^[1] d) ↔ (c [M]==> d)
+  lemma step_is_step_t_1 {c d : config rc ic}
+    : (c [P]==>^[1] d) ↔ (c [P]==> d)
     := begin split, intro h, simpa using h,
               intro h, simpa using h end
   
-  lemma steps_to_trans {c d e : state rc ic}
-    (h1 : c [M]==>* d) (h2 : d [M]==>* e)
-    : c [M]==>* e
+  lemma step_t_unique {c d e : config rc ic} {t : ℕ}
+    (h1 : c [P]==>^[t] d) (h2 : c [P]==>^[t] e)
+    : d = e
+    := begin
+      induction t generalizing c,
+      simp at *, exact eq.trans h1.symm h2,
+      simp at h1 h2,
+      refine @t_ih (step P c) _ _,
+      simpa using h1,
+      simpa using h2,
+    end
+  
+  lemma step_t_trans {c d e : config rc ic} {t1 t2 : ℕ}
+    (h1 : c [P]==>^[t1] d) (h2 : d [P]==>^[t2] e)
+    : c [P]==>^[t1+t2] e
+    := begin
+      simp at h1 h2 |-,
+      rw nat.add_comm t1 t2,
+      rw function.iterate_add_apply (step P) t2 t1 c,
+      rw [h1,h2],
+    end
+  
+  lemma steps_to_trans {c d e : config rc ic}
+    (h1 : c [P]==>* d) (h2 : d [P]==>* e)
+    : c [P]==>* e
     := begin
       cases h1, cases h2,
       use h2_w + h1_w,
       simp at h1_h h2_h,
       simp [function.iterate_add, h1_h, h2_h]
     end
+  
+  lemma halt_fix_step_t (regs : fin rc → ℕ) (t : ℕ)
+    : {ip := none, regs := regs} [P]==>^[t] {ip := none, regs := regs}
+    := begin induction t, simp, simpa, end
 
-  lemma halt_is_fixpoint (regs : vector ℕ rc)
-    : {ip := none, regs := regs} [M]==> {ip := none, regs := regs}
-    := begin simp [step] end
+  def run_from_state : config rc ic →. (fin rc → ℕ)
+    := pfun.fix (λ c, roption.some (
+        if c.is_halted  then sum.inl c.regs
+                        else sum.inr (P.step c)))
+  
+  theorem run_from_state_dom_if_steps {c : config rc ic}
+    : (∃ rs, c [P]==>* config.halted rs) → (P.run_from_state c).dom
+    := begin
+      intro h, cases h, cases h_h,
+      rw run_from_state,
+      exact sorry,
+    end
 
-  def computes (M : rm rc.succ ic.succ) (f : ℕ → ℕ) := ∀ (n : ℕ), ∃ (regs : vector ℕ rc.succ),
-    ({ip := some 0, regs := vector.of_fn (λ i, fin.cases n (λ _, 0) i)}
-      [M]==>* {ip := none, regs := regs}) ∧ regs.nth 0 = f n
+  @[simp]
+  def evals_from_to {rcp : ℕ} (P : prog rcp.succ ic) (input : ℕ) (output : ℕ) : Prop
+    := ∃ tail, config.init input [P]==>*
+                config.halted (fin.cons output tail)
+  
+  def eval {rcp : ℕ} (P : prog rcp.succ ic) : ℕ →. ℕ
+    := λ n, {dom := ∃ m, P.evals_from_to n m, get := λ h,
+              (P.run_from_state (config.init n)).get (begin
+                apply run_from_state_dom_if_steps,
+                cases h, cases h_h, use fin.cons h_w h_h_w,
+                exact h_h_h,
+              end) 0}
+
+  theorem eval_mem_iff_steps {rcp ic : ℕ} (P : prog rcp.succ ic) {n m : ℕ}
+    : m ∈ P.eval n ↔ ∃ tail, config.init n [P]==>* config.halted (fin.cons m tail)
+    := sorry
+
+
+end prog
+
+namespace prog
+  def id : prog 1 0 := ![]
+
+  theorem id.behavior (n : ℕ)
+    : (config.init n) [id]==>* (config.halted ![n])
+    := begin use 0, simp [prog.step], refl, end
+
+  def succ : prog 1 1 := λ _, instr.inc 0 none
+
+  theorem succ.behavior (n : ℕ)
+    : (config.init n) [succ]==>* (config.halted ![n.succ])
+    := begin use 1, simp [succ, prog.step, function.update],
+        rw fin.update_cons_zero, refl,
+      end
+
+  def embed {rc ic : ℕ} (P : prog rc ic) {rc' : ℕ} (f : fin rc → fin rc')
+    : prog rc' ic
+    := (instr.map_regs f) ∘ P
+  
+/-   section
+    variables {rc ic : ℕ} (P : prog rc ic) {rc' : ℕ}
+        (f : fin rc → fin rc')
+        (h : ∀ r', )
+
+    variables
+      {ip1 ip2 : fin ic} {r1 r2 : fin rc → ℕ}
+      {r1' : fin rc' → ℕ} (h : r1 = r1' ∘ f)
+
+    lemma embed_regs_preserves_step
+      (behav : ⟨ip1, r1⟩ [P]==> ⟨ip2, r2⟩)
+      : ⟨ip1, r1'⟩ [embed P f]==> ⟨ip2, embed_regs_res⟩
+      := begin end
+
+    theorem embed_regs_preserves_behavior
+      (behav : ⟨ip1, r1⟩ [P]==>* ⟨ip2, r2⟩)
+      : ⟨ip1, r1'⟩ [embed P f]==>* ⟨ip2, r2'⟩
+      := begin
+        cases behav, use behav_w,
+        induction behav_w,
+        simp at *, split, exact behav_h.1,
+        
+      end
+  end -/
+
+  def seq {rc ic1 ic2 : ℕ} (P1 : prog rc ic1) (P2 : prog rc ic2)
+    : prog rc (ic1+ic2) :=
+      fin.append
+        (rfl : ic1+ic2 = ic1+ic2)
+        (instr.map_locs (λ o : option (fin ic1), match o with
+                              | some i := some ⟨i.val, i.val.lt_add_right ic1 ic2 i.prop⟩
+                              | none := match ic2 with
+                                        | 0 := none
+                                        | ic2p+1 := some ⟨ic1, nat.add_lt_add_left fin.last_pos ic1⟩
+                                        end
+                              end)
+            ∘ P1)
+        (instr.map_locs (option.map (λ i, ⟨ic1 + i,nat.add_lt_add_left i.prop ic1⟩))
+            ∘ P2)
+
+  lemma seq.behavior {rc ic1 ic2 : ℕ} {P1 : prog rc ic1} {P2 : prog rc ic2}
+    {n : ℕ} {r1 r2 r3 : fin rc → ℕ}
+    (h1 : {ip := config.init_ip rc ic1, regs := r1} [P1]==>* config.halted r2)
+    (h2 : {ip := config.init_ip rc ic2, regs := r2} [P2]==>* config.halted r3)
+    : {ip := config.init_ip rc (ic1+ic2), regs := r1}
+          [seq P1 P2]==>* config.halted r3
+    := sorry
+
+  def loop {rc ic : ℕ} (P : prog rc ic)
+    : prog rc.succ ic.succ
+    := fin.cons (instr.dec 0 (some 1) none)
+        (instr.map_locs (λ l, match l with some x := some x.succ | none := some 0 end)
+          ∘ instr.map_regs (λ r, r.succ)
+          ∘ P)
+
+  theorem loop.behavior {rc ic : ℕ} (P : prog rc ic)
+        (f_P : (fin rc → ℕ) → (fin rc → ℕ))
+        (hf : ∀ regs, ⟨config.init_ip rc ic,regs⟩ [P]==>* {ip := none, regs := f_P regs})
+    : ∀ n regs, {ip := some 0, regs := fin.cons n regs}
+        [loop P]==>* {ip := none, regs := fin.cons 0 (f_P^[n] regs)}
+    := sorry
+
+  def reset : prog 1 1 := loop ![]
+
+  lemma reset.behavior (n : ℕ)
+    : (config.init n) [reset]==>* (config.halted (![0]))
+    := begin
+      convert loop.behavior ![] (λ x,x) (begin intro, use 0, simp, end) n ![],
+      simp,
+    end
+
+  def mov {rc : ℕ} (_fr _to : fin rc) : prog rc 2
+    := embed (loop (![instr.inc 0 none])) ![_fr, _to]
+  
+  theorem mov.behavior {rc ic : ℕ} (_fr _to : fin rc) {hr : _fr ≠ _to}
+    : sorry
+    := sorry
+end prog
+
+/- encodable type where an RM can recognize
+    valid/invalid encodings (to prevent adding
+    computational power via the encoding) -/
+class rmcodable (α : Type*)
+  := (to_encodable : encodable α)
+      {coding_rcp coding_icp : ℕ} (coding_P : prog coding_rcp.succ coding_icp.succ)
+      (h : ∀ n, (encodable.encode (encodable.decode α n)) ∈ coding_P.eval n)
+
+instance rmcodable_to_encodable {α : Type*} [rmcodable α] : encodable α
+  := rmcodable.to_encodable
+
+namespace rmcodable
+  section
+    variables {α : Type*} [c : rmcodable α]
+
+    def encode : α → ℕ := c.to_encodable.encode
+    def decode : ℕ → option α := c.to_encodable.decode
+  end
+  
+  def of_equiv {β} (α) [c : rmcodable α] (e : β ≃ α) : rmcodable β
+    := let beta_enc := encodable.of_equiv α e in
+      ⟨beta_enc, c.coding_P, begin
+        intros, have := @rmcodable.h _ c n,
+        rw prog.eval_mem_iff_steps at this |-,
+        cases this, use this_w,
+        have : encodable.encode (encodable.decode α n) = @encodable.encode _ (@encodable.option _ beta_enc) (@encodable.decode β beta_enc n),
+          simp [encodable.encode, encodable.decode],
+          cases encodable.decode α n,
+          dsimp, refl,
+          dsimp, simp,
+        rw ←this, exact this_h,
+      end⟩
+  
+  instance nat : rmcodable ℕ := ⟨encodable.nat, prog.succ, begin
+      intros, rw prog.eval_mem_iff_steps, use ![],
+      exact prog.succ.behavior n,
+    end⟩
+
+  instance fin (n) : rmcodable (fin n)
+    := ⟨encodable.fin n,
+      (sorry : prog 1 1), sorry
+    ⟩
+
+  instance prod {α β} [rmcodable α] [rmcodable β] : rmcodable (α × β)
+    := ⟨encodable.prod,
+      (sorry : prog 1 1),
+      sorry
+    ⟩
+
+  instance sum {α β} [rmcodable α] [rmcodable β] : rmcodable (α ⊕ β)
+    := ⟨encodable.sum,
+      (sorry : prog 1 1),
+      sorry
+    ⟩
+
+  instance option {α : Type*} [ae : encodable α] : rmcodable (option α)
+    := ⟨encodable.option,
+      (sorry : prog 1 1), sorry
+    ⟩
+
+  instance list {α : Type*} [ae : encodable α] : rmcodable (list α)
+    := ⟨encodable.list,
+      (sorry : prog 1 1), sorry
+    ⟩
+
+  instance instr {rc ic : ℕ} : rmcodable (instr rc ic)
+    := of_equiv _ instr.equiv_destr
+
+  instance {rc ic : ℕ} : rmcodable (prog rc ic)
+    := sorry
+
+end rmcodable
+
+def apply {rcp ic : ℕ} (P : prog rcp.succ ic)
+    {α β : Type*} [rmcodable α] [rmcodable β] : α →. β
+  := λ a, (P.eval (rmcodable.encode a)).bind
+            (roption.of_option ∘ (@rmcodable.decode β _))
+
+  /- goal: build up this universal machine
+
+  0 := copy E R 1
+  1 := write R p x 2
+  2 := read E p I 3
+  3 := pop I r 4
+  4 := zero I halt 5
+  5 := pop I p 6
+  6 := read R r x 7
+  7 := zero I 8 9
+  8 := inc x 12
+  9 := zero x 10 11
+  10 := pop I p 2
+  11 := dec x 12 12
+  12 := write R r x 2
+  -/
+
+def univ_machine : prog (nat.succ sorry) sorry := sorry
+
+theorem univ_machine_computes_eval {rcp ic : ℕ} (P : prog rcp.succ ic)
+  (n : ℕ) : apply univ_machine (P,n) = P.eval n := sorry
 
 end rm
-
-namespace subproc
-  variables {rc prelen sublen postlen : ℕ}
-            (halt_loc : option (fin (prelen + sublen + postlen)))
-
-  def embed_line (l : fin sublen)
-    : fin (prelen + sublen + postlen)
-    := fin.cast_add postlen (fin.nat_add prelen l)
-
-  def embed_loc (loc : option (fin sublen))
-    : option (fin (prelen + sublen + postlen))
-    := match loc with
-    | some l := some (embed_line l)
-    | none := halt_loc
-    end
-  
-  @[simp] def embed_state (s : state rc sublen)
-    : state rc (prelen + sublen + postlen)
-    := {ip := embed_loc halt_loc s.ip, regs := s.regs}
-
-  @[simp] def embed_rm (M : rm rc sublen)
-    : vector (instr rc (prelen + sublen + postlen)) sublen
-    := M.map (instr.map_locs (embed_loc halt_loc))
-
-  section
-  variables 
-    (preM : vector (instr rc (prelen+sublen+postlen)) prelen)
-    (subM : rm rc sublen)
-    (postM : vector (instr rc (prelen+sublen+postlen)) postlen)
-
-  lemma preserves_step
-    : let M : rm rc (prelen+sublen+postlen)
-            := (preM.append (embed_rm halt_loc subM)).append postM in
-      ∀ {c : state rc sublen},
-        (embed_state halt_loc c [M]==>* embed_state halt_loc (subM.step c))
-    := begin
-      intros,
-      cases h : c, rw h at *, clear h c,
-      cases ip,
-      have h := subM.halt_is_fixpoint regs,
-      use 0,
-      simp [h],
-      use 1,
-      rw [rm.step_t, nat.iterate, nat.iterate],
-      have : M.nth (embed_line ip) = instr.map_locs (embed_loc halt_loc) (subM.nth ip),
-        simp [embed_line, embed_loc],
-      simp [embed_loc, rm.step, this],
-      cases h : (subM.nth ip),
-      case regmachine.instr.inc : r l {
-        simp [rm.step, embed_loc],
-      },
-      case regmachine.instr.dec : r l k {
-        cases h' : regs.nth r,
-        simp [rm.step, embed_loc, h'],
-        simp [rm.step, embed_loc, h'],
-      }
-    end
-
-  theorem preserves_behavior
-    : let M : rm rc (prelen+sublen+postlen)
-            := (preM.append (embed_rm halt_loc subM)).append postM in
-      ∀ {c d : state rc sublen}, (c [subM]==>* d)
-        → (embed_state halt_loc c [M]==>* embed_state halt_loc d)
-    := begin
-      intros M c d h,
-      cases h,
-      induction h_w generalizing c,
-      simp at h_h,
-      use 0,
-      simp [h_h],
-      simp at h_h,
-      have rest := h_w_ih h_h,
-      clear h_w_ih h_h,
-      have step : (embed_state halt_loc c [M]==>* embed_state halt_loc (subM.step c))
-                := preserves_step _ _ _ _,
-      exact M.steps_to_trans step rest,
-    end
-  end
-
-end subproc
-
-end regmachine
